Add simplified definition of bdd_satcount; drafted proof

core/CountSAT.thy
@@ -3,6 +3,8 @@ theory CountSAT
 imports Data Evaluate "HOL-Library.Multiset"
 begin
 
+subsection \<open>Requests and Priority Queues\<close>
+
 datatype 'l pq_item = Request (target: \<open>'l uid\<close>) (sum: \<open>nat\<close>) (levels_visited: \<open>nat\<close>)
 
 instantiation pq_item :: (linorder) linorder
@@ -50,6 +52,8 @@ lemma top_Min:
   by (metis Min_le finite_set_mset option.discI option.sel that top_def)
 
 
+subsection \<open>Definition from Adiar\<close>
+
 context
   fixes varcount :: nat
 begin
@@ -95,6 +99,204 @@ fun bdd_satcount :: \<open>('l :: linorder) bdd \<Rightarrow> nat\<close> where
     (let (rt, pq)  = forward_paths {#} t 1 1
        ; (re, pq') = forward_paths pq e 1 1
      in bdd_satcount_acc ns pq' (rt + re))\<close>
+
+
+subsection \<open>Simplified definition\<close>
+
+fun bdd_satcount_acc' :: \<open>('l :: linorder) node list => 'l pq \<Rightarrow> nat \<Rightarrow> nat\<close> where
+  \<open>bdd_satcount_acc' [] pq result_acc =
+    (case top pq of None \<Rightarrow> result_acc
+                  | _    \<Rightarrow> undefined)\<close>
+| \<open>bdd_satcount_acc' ((N i t e) # ns) pq result_acc =
+    (case top pq of None                   \<Rightarrow> result_acc
+                  | Some (Request tgt _ v) \<Rightarrow> (if i = tgt
+                                               then let (s, lvls, pq') = (0, v, pq)\<^cancel>\<open>combine_paths pq tgt\<close>
+                                                      ; (rt, pq'') = forward_paths pq' t s (lvls+1)
+                                                      ; (re, pq''') = forward_paths pq'' e s (lvls+1)
+                                                     in bdd_satcount_acc' ns pq''' (result_acc + rt + re)
+                                               else bdd_satcount_acc' ns pq result_acc))\<close>
+
+fun bdd_satcount' :: \<open>('l :: linorder) bdd \<Rightarrow> nat\<close> where
+  \<open>bdd_satcount' (Constant False)    = 0\<close>
+| \<open>bdd_satcount' (Constant True)     = 2^varcount\<close>
+| \<open>bdd_satcount' (Nodes ((N i t e) # ns)) =
+    (let (rt, pq)  = forward_paths {#} t 1 1
+       ; (re, pq') = forward_paths pq e 1 1
+     in bdd_satcount_acc' ns pq' (rt + re))\<close>
+
+abbreviation
+  "dom_bounded n a \<equiv> a ` (UNIV - {0..<n}) \<subseteq> {False}"
+
+definition
+  "num_assignments n bdd = card {a. bdd_eval bdd a \<and> dom_bounded n a}"
+
+definition
+  "num_assignments_nl n u ns = card {a. bdd_eval_aux ns a u \<and> dom_bounded n a}"
+
+definition
+  "num_assignments_nl_ptr n ptr ns = card {a. bdd_eval_ptr ns a ptr \<and> dom_bounded n a}"
+
+
+subsection \<open>Properties of assignment counting\<close>
+
+lemma num_assignments_nl_ptr_alt_def:
+  "num_assignments_nl_ptr n ptr ns = (
+      case ptr of
+        Leaf False \<Rightarrow> 0
+      | Leaf True  \<Rightarrow> 2 ^ n
+      | Node u \<Rightarrow> num_assignments_nl n u ns
+  )"
+  sorry
+
+lemma num_assignments_Const_True:
+  "num_assignments n (Constant True) = 2 ^ n"
+  unfolding num_assignments_def apply simp
+  sorry
+
+lemma num_assignments_Const_False:
+  "num_assignments n (Constant False) = 0"
+  unfolding num_assignments_def by simp
+
+
+subsection \<open>Properties of bounded Boolean functions\<close>
+
+lemma dom_bounded_alt_def:
+  "dom_bounded n a \<longleftrightarrow> (\<forall>i. i \<notin> {0..<n} \<longrightarrow> a i = False)"
+  by blast
+
+lemma dom_bounded_minus_1_iff:
+  "dom_bounded n a \<and> a (n - 1) = False \<longleftrightarrow> dom_bounded (n - 1) a" if "n > 0" for n :: nat
+proof -
+  have "{0..<n} = {0..<n-1} \<union> {n-1}"
+    using that by auto
+  show ?thesis
+    unfolding dom_bounded_alt_def \<open>{0..<n} = _\<close> by force
+qed
+
+subsection \<open>An additional well-formedness condition on BDDs\<close>
+
+definition well_formed_node where
+  "well_formed_node \<equiv> \<lambda>N i t e \<Rightarrow>
+    (case t of Node i1 \<Rightarrow> label i < label i1 | _ \<Rightarrow> True)
+  \<and> (case t of Node i2 \<Rightarrow> label i < label i2 | _ \<Rightarrow> True)
+  "
+
+fun well_formed_nodes :: \<open>('l :: linorder) bdd \<Rightarrow> bool\<close> where
+  \<open>well_formed_nodes (Constant _) = True\<close>
+| \<open>well_formed_nodes (Nodes ns)   = list_all well_formed_node ns\<close>
+
+
+subsection \<open>The central property of recursive counting of assignments\<close>
+
+lemma num_assignments_split:
+  "num_assignments varcount (Nodes (N i t e # ns)) =
+   num_assignments_nl_ptr (varcount - 1) t ns + num_assignments_nl_ptr (varcount - 1) e ns"
+  (is "?l = ?r")
+  if "well_formed bdd" "well_formed_nodes bdd"
+proof -
+  \<comment> \<open>Need to prove these from the well-formedness assumptions\<close>
+  have "0 < varcount" "label i = varcount - 1"
+    sorry
+  have 1: "{a. (a (label i) \<longrightarrow>
+          bdd_eval_ptr ns a e \<and> dom_bounded varcount a) \<and>
+         (\<not> a (label i) \<longrightarrow>
+          bdd_eval_ptr ns a t \<and> dom_bounded varcount a)}
+  = {a. a (label i) \<and> bdd_eval_ptr ns a e \<and> dom_bounded varcount a}
+  \<union> {a. \<not> a (label i) \<and> bdd_eval_ptr ns a t \<and> dom_bounded varcount a}" (is "?S = ?Se \<union> ?St")
+    by auto
+  \<comment> \<open>Because \<open>e\<close> cannot refer to \<open>label i\<close>.\<close>
+  have "bdd_eval_ptr ns a e \<longleftrightarrow> bdd_eval_ptr ns (a(label i := b)) e" for a b
+    sorry
+  then have "card ?Se
+      = card {a. \<not> a (label i) \<and> bdd_eval_ptr ns a e \<and> dom_bounded varcount a}" (is "_ = card ?Se'")
+    apply (intro card_bij_eq[where f = "\<lambda>a. a(label i := False)" and g = "\<lambda>a. a(label i := True)"])
+    subgoal inj_on_f
+      by (smt (verit, del_insts) fun_upd_triv fun_upd_upd inj_onI mem_Collect_eq)
+    subgoal subs_A
+      by (auto simp: \<open>label i = _\<close> split: if_split_asm)
+    subgoal inj_on_g
+      by (smt (verit, del_insts) fun_upd_triv fun_upd_upd inj_onI mem_Collect_eq)
+    subgoal subs_B
+      by (auto simp: \<open>label i = _\<close> \<open>varcount > 0\<close> split: if_split_asm)
+    subgoal finite_A \<comment> \<open>Finiteness\<close>
+      sorry
+    subgoal finite_B \<comment> \<open>Finiteness\<close>
+      by (rule inj_on_finite, rule inj_on_g, assumption, rule subs_B, assumption, rule finite_A)
+    done
+  have "?St = {a. bdd_eval_ptr ns a t \<and> dom_bounded (varcount - Suc 0) a}"
+    using dom_bounded_minus_1_iff[OF \<open>varcount > 0\<close>] \<open>label i = _\<close>
+    by simp (metis (no_types, hide_lams))
+  have "?Se' = {a. bdd_eval_ptr ns a e \<and> dom_bounded (varcount - Suc 0) a}"
+    using dom_bounded_minus_1_iff[OF \<open>varcount > 0\<close>] \<open>label i = _\<close>
+    by simp (metis (no_types, hide_lams))
+  have disjoint: "?Se \<inter> ?St = {}"
+    by auto
+  have finite: "finite ?Se" "finite ?St" \<comment> \<open>Proofs of finiteness are annoying but routine.\<close>
+    sorry
+  have "?l = num_assignments_nl varcount i (N i t e # ns)"
+    unfolding num_assignments_def num_assignments_nl_def by simp
+  also have "\<dots> = card ?S"
+    unfolding num_assignments_nl_def bdd_eval_aux_Cons_alt num_assignments_nl_ptr_def by simp
+  also have "\<dots> = ?r"
+    unfolding num_assignments_nl_def bdd_eval_aux_Cons_alt num_assignments_nl_ptr_def 1
+    by (subst card_Un_disjoint, rule finite, rule finite, rule disjoint)
+       (simp add: \<open>?St = _\<close> \<open>card ?Se = _\<close> \<open>?Se' = _\<close>)
+  finally show ?thesis .
+qed
+
+
+subsection \<open>Assigning an assignment count to priority queues\<close>
+
+definition
+  "num_request ns \<equiv> \<lambda>Request u s l \<Rightarrow> s * num_assignments_nl (varcount - l) u ns"
+
+definition
+  "num_pq ns pq \<equiv> \<Sum>r \<in># pq. num_request ns r"
+
+lemma num_pq_Mempty_eq_0[simp]:
+  "num_pq ns {#} = 0"
+  unfolding num_pq_def by simp
+
+
+subsection \<open>Proving correctness of @{term bdd_satcount'}}\<close>
+
+lemma forward_pathsE:
+  obtains s' pq' where
+    "forward_paths pq ptr s l = (s', pq')"
+    "num_pq ns pq' + s' = num_pq ns pq + s * num_assignments_nl_ptr (varcount - l) ptr ns"
+  sorry
+
+lemma bdd_satcount_acc'_correct:
+  "bdd_satcount_acc' ns pq s = s + num_pq ns pq"
+  sorry
+
+theorem bdd_satcount'_correct:
+  assumes "well_formed bdd" "well_formed_nodes bdd"
+  shows "bdd_satcount' bdd = num_assignments varcount bdd"
+proof (cases bdd rule: bdd_satcount'.cases)
+next
+  case (3 i t e ns)
+  obtain rt pq where 1:
+    "forward_paths {#} t 1 1 = (rt, pq)"
+    "num_pq ns pq + rt = num_pq ns {#} + 1 * num_assignments_nl_ptr (varcount - 1) t ns"
+    by (rule forward_pathsE[of "{#}" t 1 1 ns])
+  obtain re pq' where 2:
+    "forward_paths pq e 1 1 = (re, pq')"
+    "num_pq ns pq' + re = num_pq ns pq + 1 * num_assignments_nl_ptr (varcount - 1) e ns"
+    by (rule forward_pathsE)
+  have "bdd_satcount' bdd = bdd_satcount_acc' ns pq' (rt + re)"
+    using 1 2 by (simp add: \<open>bdd = _\<close>)
+  also have "\<dots> = rt + re + num_pq ns pq'"
+    by (rule bdd_satcount_acc'_correct)
+  also have "\<dots> = num_assignments_nl_ptr (varcount - 1) t ns + num_assignments_nl_ptr (varcount - 1) e ns"
+    using 1(2) 2(2) by simp
+  also have "\<dots> = num_assignments varcount (Nodes (N i t e # ns))"
+    using assms by (rule num_assignments_split[symmetric])
+  also have "\<dots> = num_assignments varcount bdd"
+    unfolding \<open>bdd = _\<close> ..
+  finally show ?thesis .
+qed (use assms in \<open>simp_all add: num_assignments_Const_True num_assignments_Const_False\<close>)
+
 end
 
 end
